first attempt to hw 10 (a). looks not too bad.

Dependency_Template.thy
@@ -20,9 +20,89 @@ text {* The dependency relation *}
 
 inductive influences :: "name \<Rightarrow> com \<Rightarrow> name \<Rightarrow> bool"
 where
-  "influences x SKIP x"
-  (* add missing rules *)
+  Skip:       "influences x SKIP x" |
+  AssignEq:   "y \<in> (vars a) \<Longrightarrow> influences y (x ::= a) x" |
+  AssignNeq:  "y \<noteq> x \<Longrightarrow> influences y (x ::= a) y" |
+  Semi:       "\<lbrakk> influences y c1 z; influences z c2 x \<rbrakk> \<Longrightarrow> influences y (c1; c2) x" |
+  IfThen:     "influences y c1 x \<Longrightarrow> influences y (IF b THEN c1 ELSE c2) x" |
+  IfElse:     "influences y c2 x \<Longrightarrow> influences y (IF b THEN c1 ELSE c2) x" |
+  IfCondThen: "\<lbrakk> y \<in> vars b; assigned c1 x \<rbrakk> \<Longrightarrow> influences y (IF b THEN c1 ELSE c2) x" |
+  IfCondElse: "\<lbrakk> y \<in> vars b; assigned c2 x \<rbrakk> \<Longrightarrow> influences y (IF b THEN c1 ELSE c2) x" |
+  WhileSkip:  "influences x (WHILE b DO c) x" |
+  WhileCond:  "\<lbrakk> y \<in> vars b; assigned c x \<rbrakk> \<Longrightarrow> influences y (WHILE b DO c) x" |
+  WhileStep:  "\<lbrakk> influences y c x \<rbrakk> \<Longrightarrow> influences y (WHILE b DO c) x" |
+  WhileTrans: "\<lbrakk> influences y c z; influences z (WHILE b DO c) x \<rbrakk> 
+               \<Longrightarrow> influences y (WHILE b DO c) x" (* this rule might cause trouble *)
 
+(* Is there a way to execute influences? 
+
+   I can see where problems might be. For example in the Semi rule a potential
+   execution would need to guess the z. Also e.g. in IfCondThen we have
+   "assigned c1 x" where x is not yet determined, so again x would need to be
+   guessed. Maybe there is a better definition of 'influences' that allows
+   execution. However my version might still be ok for the soundness proof.
+
+   One thing one could do, is instead of the "assigned c x", we define a
+   function "assigned_vars" similar to "vars" and have "x \<in> assigned_vars c"
+   instead.
+
+   Guessing the "z" in the Semi and WhileTrans rule might be done with some
+   kind of heuristic of possible values for z. Maybe something like z is
+   either y or x or in "assigned_vars c".
+
+   I assume here that the soundness proof is not effected by this
+   shortcoming. We will see next week.
+
+   Technical question: Is there some documentation on "code_pred"? I can
+   actually execute "code_pred influences ." without error or warning or any
+   hint at all, but the values/value fail miserably.
+*)
+
+(* proof automation *)
+(* keep in mind this is potentially to aggressive use of automation *)
+inductive_cases SkipE[elim!]:   "influences y SKIP x"
+inductive_cases AssignE[elim!]: "influences y (z ::= a) x"
+inductive_cases SemiE[elim!]:   "influences y (c1; c2) x"
+inductive_cases IfE[elim!]:     "influences y (IF b THEN c1 ELSE c2) x"
+inductive_cases WhileE[elim]:   "influences y (WHILE b DO c) x"
+declare influences.intros[simp, intro]
+declare WhileTrans[simp del]
+
+
+(* Trying some examples. I have to proof manually. Automatic proof again
+   fails, I guess because the proofer would have to guess the intermediary
+   variables, that I give explicitally. Again I think with my definition of
+   'influences' there is not much we can do about that. A different definition
+   might not have this shortcoming. *)
+
+lemma "influences 2 (WHILE b DO (0 ::= (V 1); 1 ::= (V 2))) 0"
+apply (rule WhileTrans[of _ _ 1])
+apply (rule Semi[of _ _ 2])
+apply simp
+apply simp
+apply (rule WhileStep)
+apply (rule Semi[of _ _ 0]) 
+apply auto
+done
+
+lemma "influences 3 (WHILE b DO (0 ::= (V 1); 1 ::= (V 2); 2::= (V 3))) 0"
+apply (rule WhileTrans[of _ _ 2])
+apply (rule Semi[of _ _ 3])
+apply (rule Semi[of _ _ 3])
+apply simp
+apply simp
+apply simp
+apply (rule WhileTrans[of _ _ 1])
+apply (rule Semi[of _ _ 1])
+apply (rule Semi[of _ _ 2])
+apply simp
+apply simp
+apply simp
+apply (rule WhileStep)
+apply (rule Semi[of _ _ 0])
+apply (rule Semi[of _ _ 0])
+apply auto
+done
 
 text {* All dependencies of a variable *}
 abbreviation deps :: "com \<Rightarrow> name \<Rightarrow> name set" where
@@ -33,7 +113,36 @@ text {* A simple lemma that is useful later *}
 
 lemma deps_unassigned_keep:
   "\<not> assigned c x \<Longrightarrow> x \<in> deps c x"
-oops
+proof induct
+qed auto
+
+lemma deps_unassigned_neq:
+  "\<not> assigned c x \<Longrightarrow> x \<noteq> y \<Longrightarrow> \<not> y \<in> deps c x"
+apply (induct arbitrary: y)
+apply auto
+apply metis
+proof -
+  fix b c y
+  {
+    assume "\<And> z. x\<noteq>z \<Longrightarrow> \<not> influences z c x"
+    assume "\<not> assigned c x"
+    assume "x \<noteq> y"
+    
+    have "\<not> influences y (WHILE b DO c) x"
+  } 
+  from this show "\<lbrakk>\<And>z. x \<noteq> z \<Longrightarrow> \<not> influences z c x; \<not> assigned c x; x \<noteq> y;
+    influences y (WHILE b DO c) x\<rbrakk> \<Longrightarrow> False" by blast
+qed
+
+
+lemma deps_unassigned_singelton:
+  "\<not> assigned c x \<Longrightarrow> {x} = deps c x"
+
+
+ 
+
+
+
 
 text {* Main theorem *}
 
